base/base64.mli
@@ -1,1 +1,2 @@
 val encode : string -> string
+val decode : string -> string
