coq/Base64.v
@@ -3,16 +3,7 @@ Require Import Ascii.
 Require Import Grp.
 Require Import ListUtil.
 Require Import Vec.
-(*
-Variable gfill : forall{A:Set}(default:A)(n:nat) (xs:list A) (H:0<n), list (Vec A n).
-Variable gcut : forall{A:Set} (default:A)n (xs:list A) (H:0<n), list(Vec A n).
-Variable cm : forall {A:Set}{n:nat} (vs :list (Vec A n)), list A.
-*)
 
-(*
-Axiom grp_inv: forall {A:Set}(default:A) n m H0 H1 (vs: list (Vec A m)),
-  n < m -> gcut default m (cm (gfill default n (cm vs) H0)) H1 = vs.
-*)
 Definition ascii_of_bool6 (bs: Vec bool 6) : ascii.
  intro bs.
  inversion bs.
@@ -21,9 +12,19 @@ Definition ascii_of_bool6 (bs: Vec bool 6) : ascii.
  inversion H7.
  inversion H10.
  inversion H13.
-(* exact (Ascii false false H0 H3 H6 H9 H12 H15).*)
  exact (Ascii H15 H12 H9 H6 H3 H0 false false).
 Defined.
+
+Definition bool6_of_ascii (c : ascii) : (Vec bool 6) :=
+  match c with
+    | Ascii a b c d e f _ _ =>
+      vec_of_list 6 (f::e::d::c::b::a::nil) (refl_equal _)
+  end.
+
+Lemma ascii_bool6_inv : forall bs : Vec bool 6,
+  (bool6_of_ascii (ascii_of_bool6 bs)) = bs.
+Proof.
+Admitted.
 
 Definition ascii_of_bool8 (bs: Vec bool 8) : ascii.
  intro bs.
@@ -36,11 +37,20 @@ Definition ascii_of_bool8 (bs: Vec bool 8) : ascii.
  inversion H16.
  inversion H19.
  exact (Ascii H21 H18 H15 H12 H9 H6 H3 H0).
-(* exact (Ascii H0 H3 H6 H9 H12 H15 H18 H21).*)
 Defined.
 
 Require Import Arith.
-Infix "<=?" := le_lt_dec (at level 60).
+Definition le_lt_dec_aux: forall x y:nat, {x <= y} + {~x <= y}.
+ refine (fun x y =>
+   if le_lt_dec x y then
+     left _ _
+   else
+     right _ _).
+  exact _H.
+
+  exact (lt_not_le y x _H).
+Defined.
+Infix "<=?" := le_lt_dec_aux (at level 60).
 Infix "=?" := eq_nat_dec (at level 60).
 
 Definition tblaux (n: nat) : nat :=
@@ -58,12 +68,25 @@ Definition tblaux (n: nat) : nat :=
 Definition tbl (bs: Vec bool 6) : ascii :=
   ascii_of_nat (tblaux (nat_of_ascii (ascii_of_bool6 bs))).
 
-Variable tbl_inv : (ascii) -> Vec bool 6.
+Definition tblaux_inv (n: nat) : nat :=
+  if 97 <=? n then (* n is ['a'..'z'] *)
+    26 + n - nat_of_ascii "a"
+  else if 65 <=? n then (* n is ['A'..'Z'] *)
+    n - nat_of_ascii "A"
+  else if 48 <=? n then (* n is ['0'..'9'] *)
+    52 + n - nat_of_ascii "0"
+  else if n =? nat_of_ascii "+" then
+    62
+  else (* if n = nat_of_ascii "/" *) 
+    63.
+
+Definition tbl_inv (c: ascii) : Vec bool 6 :=
+  bool6_of_ascii (ascii_of_nat (tblaux_inv (nat_of_ascii c))).
 
 Definition digit (char:ascii) : Vec bool 8 :=
   match char with
-    | Ascii a b c d e f g h => vec_of_list 8 (h::g::f::e::d::c::b::a::nil) (refl_equal _)
-(*    | Ascii a b c d e f g h => vec_of_list 8 (a::b::c::d::e::f::g::h::nil) (refl_equal _)*)
+    | Ascii a b c d e f g h =>
+      vec_of_list 8 (h::g::f::e::d::c::b::a::nil) (refl_equal _)
   end.
 
 Definition digits : list ascii -> list (Vec bool 8) := map digit.
@@ -81,9 +104,8 @@ Fixpoint string_of_list cs :=
 *)
 Require Import Extr.
 
-Axiom mlstring_inv : forall cs, asciilist_of_mlstring (mlstring_of_asciilist cs) = cs.
-Axiom mlstring_inv2: forall s,  mlstring_of_asciilist (asciilist_of_mlstring s) = s.
-
+Axiom mlstring_of_asciilist_inv : forall cs, asciilist_of_mlstring (mlstring_of_asciilist cs) = cs.
+Axiom asciilist_of_mlstring_inv : forall s,  mlstring_of_asciilist (asciilist_of_mlstring s) = s.
 
 Definition encode (s : mlstring) : mlstring :=
   mlstring_of_asciilist (cm (gfill "="%char 4 (map tbl (gfill false 6 (cm (map digit (asciilist_of_mlstring s))) (lt_O_Sn _))) (lt_O_Sn _))).
@@ -95,12 +117,111 @@ Definition decode (s: mlstring) : mlstring :=
 (*  string_of_list (map ascii_of_bool8 (gcut 8 (cm (map tbl_inv
     (delete ascii_dec "="%char (list_of_string s))))(lt_O_Sn _))).*)
 
+Lemma delete_gfill: forall d n H cs,
+  ~In d cs -> delete ascii_dec d (cm (gfill d n cs H)) = cs.
+Proof.
+ intros; simpl.
+ unfold gfill.
+ rewrite cm_dist.
+ simpl cm at 2.
+ rewrite list_vec.
+ rewrite <- app_nil_end.
+ rewrite <- app_ass.
+ rewrite cm_g1_g2.
+ rewrite delete_dist.
+ rewrite (delete_notIn _ _ _ H0).
+ rewrite delete_replicate.
+ rewrite <- app_nil_end; reflexivity.
+Qed.
 
-Axiom delete_gfill: forall d n cs H,
-~In d cs -> delete ascii_dec d (cm (gfill d n cs H)) = cs.
+Lemma ascii_nat_embedding_inv : forall n,
+  n < 256 -> nat_of_ascii (ascii_of_nat n) = n.
+Admitted.
 
-Axiom tbl_inv_inv: forall c, tbl_inv (tbl c) = c.
+Require Omega.
+Lemma tblaux_lt_256 : forall n:nat, tblaux n < 256.
+Proof.
+ unfold tblaux; intro n.
+ destruct (n <=? 25);
+   [ | destruct (n <=? 51);
+     [ | destruct (n <=? 61);
+       [ | destruct (n =? 62)
+       ]]]; simpl; omega.
+Qed.
 
+Lemma sumbool_rewrite : forall {P: Prop} (b: {P}+{~P}),
+  P -> exists H, b = left _ H.
+Proof.
+ intros P b H.
+ destruct b.
+  exists p; reflexivity.
+
+  elim n; apply H.
+Qed.
+
+Lemma sumbool_rewrite_not : forall {P: Prop} (b: {P}+{~P}),
+  ~P -> exists H, b = right _ H.
+Proof.
+ intros P b H.
+ destruct b.
+  elim H; apply p.
+
+  exists n; reflexivity.
+Qed.
+ 
+Lemma tblaux_inv_inv: forall n: nat,
+  n < 64 -> tblaux_inv (tblaux n) = n.
+Proof.
+ intros n H.
+ unfold tblaux.
+ destruct (n <=? 25).
+  unfold tblaux_inv.
+  elim (sumbool_rewrite_not (97 <=? nat_of_ascii "A" + n)); [|simpl; omega].
+  intros _H0 eq; rewrite eq.
+  elim (sumbool_rewrite (65 <=? nat_of_ascii "A" + n)); [|simpl; omega].
+  intros _H1 eq1; rewrite eq1.
+  simpl; omega.
+
+  destruct (n <=? 51).
+   unfold tblaux_inv.
+   elim (sumbool_rewrite (97 <=? nat_of_ascii "a" + (n - 26))); [|simpl; omega].
+   intros _H0 eq0; rewrite eq0.
+   simpl; omega.
+
+   destruct (n <=? 61).
+    unfold tblaux_inv.
+    elim (sumbool_rewrite_not (97 <=? nat_of_ascii "0" + (n-52))); [|simpl; omega].
+    intros _H0 eq; rewrite eq.
+    elim (sumbool_rewrite_not (65 <=? nat_of_ascii "0" + (n-52))); [|simpl; omega].
+    intros _H1 eq1; rewrite eq1.
+    elim (sumbool_rewrite (48 <=? nat_of_ascii "0" + (n-52))); [|simpl; omega].
+    intros _H2 eq2; rewrite eq2.
+    simpl; omega.
+    
+    destruct (n =? 62).
+     rewrite e; reflexivity.
+
+     unfold tblaux_inv; simpl. omega.
+Qed.
+
+Lemma nat_of_bool6_lt_64: forall bs: Vec bool 6,
+  nat_of_ascii (ascii_of_bool6 bs) < 64.
+Admitted.
+
+Lemma tbl_inv_inv: forall bs: Vec bool 6, tbl_inv (tbl bs) = bs.
+Proof.
+ unfold tbl.
+ unfold tbl_inv.
+ intro; rewrite ascii_nat_embedding_inv.
+  rewrite tblaux_inv_inv.
+   rewrite ascii_nat_embedding.
+    apply ascii_bool6_inv.
+    
+    apply nat_of_bool6_lt_64.
+
+   apply tblaux_lt_256.
+Qed.
+ 
 Lemma digit_inv: forall c, ascii_of_bool8 (digit c) = c.
 Proof.
  destruct c; reflexivity.
@@ -126,7 +247,7 @@ Qed.
 Theorem soundness : forall s, decode (encode s) = s.
 Proof.
  intro s; unfold encode; unfold decode.
- rewrite mlstring_inv.
+ rewrite mlstring_of_asciilist_inv.
  rewrite delete_gfill.
   rewrite map_map.
   rewrite (map_ext  _ (fun x => x) tbl_inv_inv).
@@ -135,7 +256,7 @@ Proof.
   rewrite map_map.
   rewrite (map_ext _ (fun x => x) digit_inv).
   rewrite map_id.
-  rewrite mlstring_inv2.
+  rewrite asciilist_of_mlstring_inv.
   reflexivity.
 
   apply tbl_notIn_eq.
@@ -143,5 +264,4 @@ Qed.
 
 Definition mlstring_of_string s := mlstring_of_asciilist (list_of_string s).
 
-Extraction "base64.ml" encode.
-
+Extraction "base64.ml" encode decode.
